Checkpoint before refines_to_same transfer

src/Layer2.v
@@ -6,16 +6,16 @@ Close Scope pred_scope.
 Set Implicit Arguments.
 
 Section Layer2.
-
+(*
   Definition disk2 := @mem addr addr_dec sealed_value.
   Definition state2 := (user * oracle * disk2 * store)%type.
   Definition get_user (st: state2) := fst (fst (fst st)).
   Definition get_oracle (st: state2) := snd (fst (fst st)).
   Definition get_disk (st: state2) := snd (fst st).
   Definition get_store (st: state2) := snd st.
-  
+  *)
   Inductive exec2 :
-    forall T, state2 -> prog_limited T -> @Result state2 T -> Prop :=
+    forall T, state -> prog_limited T -> @Result state T -> Prop :=
   | Exec2Finished :
       forall T (p: prog_limited T) u o d dh s o' d' dh' s' r,
       exec_limited (u, o, d, s) p (Finished (u, o', d', s') r) ->
@@ -29,8 +29,9 @@ Section Layer2.
       rep dh' d' ->
       exec2 (u, o, dh, s) p (Crashed (u, o', dh', s')).
 
-  Definition prog2_LTS := {| State:= state2; Op:= prog_limited; transition := exec2 |}.
+  Definition prog2_LTS := {| State:= state; Op:= prog_limited; transition := exec2 |}.
 
+  (*
   Definition state_equivalent_for u (st1 st2: state2) :=
   let '(u1, o1, d1, s1) := st1 in
   let '(u2, o2, d2, s2) := st2 in
@@ -55,8 +56,9 @@ Section Layer2.
      state_equivalent_for u s1' s2'
     | _, _ => False
     end.
+   *)
   
-  Definition state_noninterference {T} (p: prog_limited T) (valid: state2 -> Prop):=
+  Definition state_noninterference {T} (p: prog_limited T) (valid: state -> Prop):=
   forall viewer st1 st1' st2,
     valid st1 ->
     valid st2 ->
@@ -66,7 +68,7 @@ Section Layer2.
       exec2 st2 p st2' /\
       return_state_equivalent_for viewer st1' st2'.
 
-  Definition ret_noninterference {T} (p: prog_limited T) (valid: state2 -> Prop) :=
+  Definition ret_noninterference {T} (p: prog_limited T) (valid: state -> Prop) :=
     forall st1 st1' st2,
     valid st1 ->
     valid st2 ->
@@ -76,8 +78,7 @@ Section Layer2.
       exec2 st2 p st2' /\
       return_equivalent_for (get_user st1) st1' st2'.
 
-  Definition data_noninterference {T} (p: prog_limited T) (valid: state2 -> Prop) :=
+  Definition data_noninterference {T} (p: prog_limited T) (valid: state -> Prop) :=
     state_noninterference p valid /\
     ret_noninterference p valid.
-
 End Layer2.
