src/LayerTransfer.v
@@ -13,13 +13,7 @@ Section LayerTransfer.
     P t2 ->
     exists t1, R t1 t2.
 
-Definition simulation_preserving {T1 T2: Type} (S1: T1 -> T1 -> Prop) (S2: T2 -> T2 -> Prop)(R: T1 -> T2 -> Prop) :=
-  forall t1 t1' t2 t2',
-    R t1 t2 ->
-    R t1' t2' ->
-    S1 t1 t1' <-> S2 t2 t2'.
-    
-  Definition refines_to (s1 : state) (s2: state2) :=
+  Definition refines_to (s1 s2: state) :=
     Prog.get_user s1 = get_user s2 /\
     Prog.get_oracle s1 = get_oracle s2 /\
     rep (get_disk s2) (Prog.get_disk s1) /\
@@ -33,7 +27,7 @@ Definition simulation_preserving {T1 T2: Type} (S1: T1 -> T1 -> Prop) (S2: T2 ->
 
   
   Ltac simpl_states:=
-    unfold state, state2 in *; destruct_pairs; simpl in *.
+    unfold state in *; destruct_pairs; simpl in *.
 
   Definition refines_to_same st1 st2 := exists sr, refines_to st1 sr /\ refines_to st2 sr.
 
@@ -47,58 +41,21 @@ Definition simulation_preserving {T1 T2: Type} (S1: T1 -> T1 -> Prop) (S2: T2 ->
       cleanup; eauto.
     Qed.
 
-    Lemma exec_deterministic_oracle:
-      forall T (p: prog T) st1 st2 st1' st2' tr1 tr2,
-        exec st1 p st1' tr1 ->
-        exec st2 p st2' tr2 ->
-        Prog.get_oracle st1 = Prog.get_oracle st2 ->
-        Prog.get_oracle (extract_state st1') = Prog.get_oracle (extract_state st2').
-    Proof.
-      unfold Prog.get_oracle;
-        induction p; intros; simpl in *;
-          simpl_states; cleanup;
-            invert_exec; invert_exec;
-              cleanup; simpl in *;
-          cleanup; eauto;
-      try match goal with
-      |[H: _ :: _ = _ :: _ |- _] =>
-       inversion H; eauto
-          end.      
-      simpl_states; cleanup.
-   Abort.
-
-  
-  Lemma exec_limited_preserves_refinement:
-      forall T (p: prog_limited T)  st1 st2 st1' st2',
+    Lemma exec_limited_preserves_user:
+      forall T (p: prog_limited T) st1 st1',
         exec_limited st1 p st1' ->
-        exec_limited st2 p st2' ->
-        refines_to_same st1 st2 ->
-        refines_to_same (extract_state st1') (extract_state st2').
-  Proof.
-    unfold refines_to_same, refines_to;
-      induction p; simpl in *;
-        intros; simpl_refines_to; simpl_states; cleanup.
-    
-    - inversion H; sigT_eq; clear H;
-        inversion H0; sigT_eq; clear H0;
-          simpl_states.
-      edestruct alloc_ok; eauto.
-      apply pimpl_star_emp; eauto.
-      destruct H; cleanup.
-      destruct_lift H1.
-      edestruct alloc_ok; [| apply H6 | eauto].
-      apply pimpl_star_emp; eauto.
-      destruct H1; cleanup.
-      destruct_lift H3.
-      destruct H8, H11; cleanup.
-  Admitted.
-  
-  Lemma rep_equivalent_for:
+        Prog.get_user st1 = Prog.get_user (extract_state st1').
+    Proof.
+      induction 1; simpl in *; eauto.
+      eapply exec_preserves_user; eauto.
+    Qed.
+
+    Lemma rep_equivalent_for_fst_low:
       forall u d1 d2 d1' d2',
-        equivalent_for_fst u d1 d1' ->
+        @equivalent_for_fst _ addr_dec _ u d1 d1' ->
         rep d2 d1 ->
         rep d2' d1' ->
-        equivalent_for u d2 d2'.
+        @equivalent_for_fst _ addr_dec _ u d2 d2'.
     Proof.
       unfold equivalent_for, equivalent_for_fst, rep; intros.
       destruct_lift H0; destruct_lift H1; cleanup.
@@ -131,7 +88,7 @@ Definition simulation_preserving {T1 T2: Type} (S1: T1 -> T1 -> Prop) (S2: T2 ->
       right; do 2 eexists; intuition eauto; simpl in *.
       omega.
 
-      destruct a; [|intuition].
+                             destruct a; [|intuition].
       destruct Hx; cleanup.
       erewrite ptsto_valid in H2; [| pred_apply; cancel]; cleanup.
       
@@ -149,43 +106,17 @@ Definition simulation_preserving {T1 T2: Type} (S1: T1 -> T1 -> Prop) (S2: T2 ->
     Qed.
 
     
-    Theorem RS_right_total_filtered :
-      right_total_filtered refines_to (fun d2 => exists d1, rep (get_disk d2) d1).
-    Proof.
-      unfold state, state2, refines_to, right_total_filtered; intros;
-      simpl_refines_to; simpl_states; cleanup.
-      exists (x, x0, x3, x2); destruct_pairs; intuition eauto.
-    Qed.
-
-    Lemma RS_simulation_preserving:
-      forall u, simulation_preserving refines_to_same (state_equivalent_for u) refines_to.
-    Proof.
-      unfold simulation_preserving, refines_to_same, refines_to,
-      Prog.state_equivalent_for, state_equivalent_for; intros.
-      simpl_refines_to; simpl_states; cleanup.
-      split; intros; cleanup; intuition.
-      admit.
-      admit.
-
-      exists(x, x0, x1, x2); intuition eauto.
-      simpl in *.
-    Abort.
-  
-    
-  
-
-    
-
-    Lemma exec_preserves_rep:
-      forall T (p: prog2 T)  st1 d1 st1' tr,
-        exec st1 (prog2_to_prog p) st1' tr ->
+    Lemma exec_limited_preserves_rep:
+      forall T (p: prog_limited T)  st1 d1 st1',
+        exec_limited st1 p st1' ->
         rep d1 (Prog.get_disk st1) ->
         exists d1', rep d1' (Prog.get_disk (extract_state st1')).
     Proof.
       induction p; intros; cleanup; simpl in *; eauto;
-      unfold Prog.get_disk, state in *; destruct_pairs; simpl in *.
+        unfold Prog.get_disk, state in *; destruct_pairs; simpl in *;
+      try (inversion H; sigT_eq); simpl in *.
       - edestruct alloc_ok; eauto.
-        apply pimpl_star_emp; eauto.
+        apply pimpl_star_emp; eauto.       
         destruct H1; cleanup;
         destruct_lift H3; eauto.
 
@@ -206,85 +137,114 @@ Definition simulation_preserving {T1 T2: Type} (S1: T1 -> T1 -> Prop) (S2: T2 ->
         
       - invert_exec; cleanup; simpl in *; eauto.
 
-      - invert_exec.
-        eapply IHp in H0; eauto; cleanup; simpl in *.
-        eapply H in H2; eauto; cleanup; simpl in *.
+      - inversion H0; sigT_eq; simpl in *.
+        invert_exec.
+        edestruct IHp; eauto; cleanup; simpl in *.
+        econstructor; eauto.
+        simpl; eauto.
+        simpl in *.
+
+        edestruct H; eauto; cleanup; simpl in *.
+        econstructor; eauto.
+        simpl; eauto.
         
-        destruct H0; cleanup; simpl in *.
-        eapply IHp in H0; eauto; cleanup; simpl in *.
-        eapply IHp in H0; eauto; cleanup; simpl in *.
-        eapply H in H2; eauto; cleanup; simpl in *.
+        destruct H6; cleanup; simpl in *.
+        edestruct IHp; eauto; cleanup; simpl in *.
+        econstructor; eauto.
+        simpl; eauto.
+        simpl; eauto.
+
+        edestruct IHp; eauto; cleanup; simpl in *.
+        econstructor; eauto.
+        simpl; eauto.
+        simpl in *.
+
+        edestruct H; eauto; cleanup; simpl in *.
+        econstructor; eauto.
+        simpl; eauto.
     Qed.
 
     
 
-    Theorem RS_strong_bisimulation:
-      StrongBisimulation prog_LTS prog2_LTS RP RS.
-    Proof.
-      unfold RP, RS; constructor; intros.
-      cleanup; simpl in *.
-      unfold Prog.get_user, get_user,
-        Prog.get_oracle, get_oracle,
-        Prog.get_disk, get_disk,
-        Prog.get_store, get_store in *; simpl in *; cleanup.
-      unfold state, state2 in *; destruct_pairs; simpl in *.
-      split; intros.
+  Definition prog_eq T (p1: Op prog_limited_LTS T) (p2: Op prog2_LTS T) := p1 = p2.
 
-      - inversion H; sigT_eq.
-        eapply_fresh exec_preserves_rep in H5; cleanup; simpl in *; eauto.
-        eapply_fresh exec_preserves_user in H5; simpl in *; cleanup.
-        destruct s1'; simpl in *; destruct_pairs; cleanup.
-        unfold Prog.get_user, Prog.get_disk in *; simpl in *; cleanup.
-        eexists; intuition.
-        econstructor; eauto.
-        all: simpl; eauto.
+  Definition refines_to_something st1 := exists st2, refines_to st1 st2.
+  Definition something_refines_to st2 := exists st1, refines_to st1 st2.
 
-        unfold Prog.get_user, Prog.get_disk in *; simpl in *; cleanup.
-        eexists; intuition.
-        eapply Exec2Crashed; simpl; eauto.
-        all: simpl; eauto.
+  Lemma exec_limited_preserves_refines_to_something:
+      forall T (p: prog_limited T)  st1 st1',
+        exec_limited st1 p st1' ->
+        refines_to_something st1 ->
+        refines_to_something (extract_state st1').
+  Proof.
+    unfold refines_to_something; intros.
+    simpl_refines_to; simpl_states; cleanup.
+    eapply exec_limited_preserves_rep in H; eauto; cleanup.
+    unfold get_disk in *.
+    simpl_states; cleanup.
+    exists(fst (fst (fst (extract_state st1'))), snd (fst (fst (extract_state st1'))), x, snd (extract_state st1'));
+      intuition eauto.
+  Qed.
 
-      - inversion H; sigT_eq.
-        simpl in *; eexists; intuition.
-    Abort.
-     *)
+  Lemma return_state_equivalent_for_refines_to:
+    forall T u (x y a b: @Result state T),
+      refines_to (extract_state x) (extract_state y) ->
+      result_same x y ->
+      result_same a b ->
+      return_state_equivalent_for u x a ->
+      refines_to (extract_state a) (extract_state b) ->
+      return_state_equivalent_for u y b.
+  Proof.
+    unfold return_state_equivalent_for, result_same, state_equivalent_for; intros.
+    simpl_refines_to; simpl_states; cleanup; intuition.
+    simpl_states; cleanup.
+    intuition.
+    eapply rep_equivalent_for_fst_low; eauto.
+    simpl_states; cleanup.
+    intuition.
+    eapply rep_equivalent_for_fst_low; eauto.
+  Qed.
 
-    Theorem transfer_low_to_high_self :
-  forall T (p: prog2 T),
-   ->
-  StrongBisimulation prog_LTS prog2_LTS RP RS ->
-  (forall T, right_total (@RP T)) ->
-  right_total_filtered RS (fun d2 => exists d1, rep (get_disk d2) d1) ->
-  (forall u, simulation_preserving (Prog.state_equivalent_for u) (state_equivalent_for u) RS) ->
-  data_noninterference p (fun d2 => exists d1, rep (get_disk d2) d1).
-Proof.
+  Lemma return_equivalent_for_refines_to:
+    forall T u (x y a b: @Result state T),
+      refines_to (extract_state x) (extract_state y) ->
+      result_same x y ->
+      result_same a b ->
+      (forall def : T, extract_ret def x = extract_ret def y) ->
+      (forall def : T, extract_ret def a = extract_ret def b) ->
+      return_equivalent_for u x a ->
+      refines_to (extract_state a) (extract_state b) ->
+      return_equivalent_for u y b.
+  Proof.
+    unfold return_equivalent_for, result_same, state_equivalent_for; intros.
+    simpl_refines_to; simpl_states; cleanup; intuition.
+    simpl_states; cleanup.
+    intuition.
+    eapply rep_equivalent_for_fst_low; eauto.
+    simpl_states; intuition; cleanup; eauto.
+    simpl_states; cleanup; intuition.   
+    eapply rep_equivalent_for_fst_low; eauto.
+  Qed.
 
+(*
   Theorem transfer_low_to_high_self :
-  forall T (p: prog2 T),
-  Prog.data_noninterference (prog2_to_prog p) (fun d1 => exists d2, rep d2 (Prog.get_disk d1)) ->
-  StrongBisimulation prog_LTS prog2_LTS RP RS ->
-  (forall T, right_total (@RP T)) ->
-  right_total_filtered RS (fun d2 => exists d1, rep (get_disk d2) d1) ->
-  (forall u, simulation_preserving (Prog.state_equivalent_for u) (state_equivalent_for u) RS) ->
-  data_noninterference p (fun d2 => exists d1, rep (get_disk d2) d1).
+  forall T (p: prog_limited T) valid_l valid_h refines_to,
+  data_noninterference p valid_l ->
+  StrongBisimulation prog_limited_LTS prog2_LTS prog_eq refines_to ->
+  (forall u, simulation_preserving (Prog.state_equivalent_for u) (state_equivalent_for u) refines_to) ->
+  data_noninterference p valid_h.
 Proof.
-  unfold right_total, right_total_filtered, simulation_preserving, result_same; intros.
+  unfold something_refines_to, refines_to_something, simulation_preserving, result_same, prog_eq; intros.
   destruct H, H0.
-  rename H1 into right_total_op.
-  rename H2 into right_total_state.
-  rename H3 into simulation_preserving.
+  rename H1 into simulation_preserving.
 
   unfold data_noninterference; split.
   - unfold state_noninterference; intros.
-    edestruct (right_total_state st1), (right_total_state st2); eauto.
-    edestruct (right_total_op T p).
-    eapply_fresh strong_bisimulation_correct0 in H5; eauto; cleanup; simpl in *.
-    apply H9 in H2; cleanup; clear H8 H9.
+    destruct 
+    eapply_fresh strong_bisimulation_correct in H3; eauto; cleanup; simpl in *.
 
-    inversion H2; sigT_eq.
-    unfold Prog.state_noninterference, Prog.ret_noninterference in *.
-    unfold RP in *; cleanup.
-    eapply_fresh H in H15; eauto; cleanup.
+    eapply_fresh H in H3 cleanup.
+    simpl_refines_to; simpl_states; cleanup; eauto.
     eapply_fresh strong_bisimulation_correct0 in H6; eauto; cleanup; simpl in *.
     edestruct H9; [econstructor; eauto|]; cleanup.
     eexists; intuition eauto.
@@ -333,3 +293,323 @@ Proof.
      pose proof H5 as Hx; unfold RS in H5; simpl in *; cleanup; eauto.
      eapply simulation_preserving; eauto.
 Qed.
+
+
+*)
+
+
+Definition simulation_preserving_right_to_left {T1 T2: Type} (S1: T1 -> T1 -> Prop) (S2: T2 -> T2 -> Prop)(R: T1 -> T2 -> Prop) :=
+  forall t1 t1' t2 t2',
+    R t1 t2 ->
+    R t1' t2' ->
+    S2 t2 t2' -> S1 t1 t1'.
+
+Lemma test:
+  (forall u, SelfSimulation prog_limited_LTS (Prog.state_equivalent_for u)) ->
+  SelfSimulation prog_limited_LTS refines_to_same.
+Proof.
+  intros; constructor; intros; simpl in *.
+  eapply_fresh H in H0.
+  simpl in *; eauto; cleanup.
+  eexists; intuition eauto.
+Abort.
+  
+
+  Theorem transfer_low_to_high_self :
+  forall T (p: prog_limited T),
+  ProgLimited.data_noninterference p refines_to_something ->
+  StrongBisimulation prog_limited_LTS prog2_LTS prog_eq refines_to ->
+  (forall u, simulation_preserving_right_to_left (Prog.state_equivalent_for u) (state_equivalent_for u) refines_to) ->
+  data_noninterference p something_refines_to.
+Proof.
+  unfold something_refines_to, refines_to_something, simulation_preserving_right_to_left, result_same, prog_eq; intros.
+  destruct H, H0.
+  rename H1 into simulation_preserving.
+
+  unfold data_noninterference; split.
+  - unfold state_noninterference; intros; cleanup.
+    eapply_fresh strong_bisimulation_correct in H3; eauto; cleanup; simpl in *.
+
+    edestruct H.
+    eexists; apply H0.
+    eexists; apply H1.
+    eauto.
+
+    (* eq_h -> eq_l required here *)
+    eapply simulation_preserving; eauto.
+    cleanup.
+
+    (* exec_limited preserves refines_to_something required in here *)
+    eapply_fresh exec_limited_preserves_refines_to_something in H9; unfold refines_to_something in *;
+      eauto; cleanup.
+    eapply_fresh exec_limited_preserves_user in H9; unfold get_user in *; simpl in *; cleanup.
+                                                                                  
+    destruct x2.
+    + simpl_states; cleanup; eauto.
+      eexists; split.
+      simpl_refines_to; cleanup.
+      econstructor; eauto.
+      simpl_refines_to; cleanup.
+      eapply return_state_equivalent_for_refines_to; eauto;
+        simpl_refines_to; intuition eauto.
+      
+    + simpl_states; cleanup; eauto.
+      eexists; split.
+      simpl_refines_to; cleanup.
+      eapply Exec2Crashed; eauto.
+      simpl_refines_to; cleanup.
+      eapply return_state_equivalent_for_refines_to; eauto;
+        simpl_refines_to; intuition eauto.
+
+  - unfold ret_noninterference; intros; cleanup.
+    eapply_fresh strong_bisimulation_correct in H3; eauto; cleanup; simpl in *.
+
+    edestruct H2.
+    eexists; apply H0.
+    eexists; apply H1.
+    eauto.
+    
+    (* eq_h -> eq_l required here *)
+    eapply simulation_preserving; eauto.
+    simpl_refines_to; cleanup; eauto.
+    cleanup.
+
+    (* exec_limited preserves refines_to_something required in here *)
+    eapply_fresh exec_limited_preserves_refines_to_something in H9; unfold refines_to_something in *;
+      eauto; cleanup.
+    eapply_fresh exec_limited_preserves_user in H9; unfold get_user in *; simpl in *; cleanup.
+                                                                                  
+    destruct x2.
+    + simpl_states; cleanup; eauto.
+      eexists; split.
+      simpl_refines_to; cleanup.
+      econstructor; eauto.
+      eapply return_equivalent_for_refines_to.
+      6: simpl_refines_to; cleanup; eauto.
+      all: simpl; eauto.
+      simpl_refines_to; cleanup; intuition eauto.
+      
+    + simpl_states; cleanup; eauto.
+      eexists; split.
+      simpl_refines_to; cleanup.
+      eapply Exec2Crashed; eauto.
+      eapply return_equivalent_for_refines_to.
+      6: simpl_refines_to; cleanup; eauto.
+      all: simpl; eauto.
+      simpl_refines_to; cleanup; intuition eauto.
+Qed.  
+
+
+Lemma exec_limited_preserves_refinement:
+      forall T (p: prog_limited T)  st1 st2 st1',
+        exec_limited st1 p st1' ->
+        refines_to_same st1 st2 ->
+        exists st2',
+          exec_limited st2 p st2' /\
+          result_same st1' st2' /\
+          refines_to_same (extract_state st1') (extract_state st2') /\
+          (forall def : T, extract_ret def st1' = extract_ret def st2').
+  Proof.
+    unfold refines_to_same; induction p; simpl in *;
+        intros; cleanup.
+    
+    - inversion H; sigT_eq; clear H;
+          simpl_states.
+      edestruct alloc_ok; eauto.
+      apply pimpl_star_emp; eauto.
+      simpl_refines_to; cleanup; eauto.
+
+      destruct H; cleanup; destruct_lifts.
+      + destruct H7; cleanup.
+        simpl_refines_to; cleanup.
+      (* needs complete correctness *)
+  Admitted.
+
+  Lemma rep_trans:
+    forall a b c,
+      rep a b ->
+      rep c b ->
+      rep c =p=> rep a.
+  Proof.
+    unfold rep; intros.
+    destruct_lift H.
+    destruct_lift H0.
+    norm. cancel.
+    intuition eauto.
+  Admitted.
+
+  Theorem RS_strong_bisimulation:
+      StrongBisimulation prog_limited_LTS prog2_LTS prog_eq refines_to.
+    Proof.
+      unfold prog_eq; constructor; intros.
+      cleanup; simpl in *.
+      split; intros.
+
+      - eapply_fresh exec_limited_preserves_rep in H; cleanup; simpl in *; eauto.
+        eapply_fresh exec_limited_preserves_user in H; simpl in *; cleanup.
+        destruct s1'; simpl_refines_to; simpl_states; cleanup.
+        eexists; intuition.
+        econstructor; eauto.
+        all: simpl; eauto.
+        
+        eexists; intuition.
+        eapply Exec2Crashed; simpl; eauto.
+        all: simpl; eauto.
+
+        simpl_refines_to; cleanup; eauto.
+        
+      - inversion H; sigT_eq; clear H.
+        simpl_refines_to; simpl_states; cleanup.
+        eapply exec_limited_preserves_refinement in H3; unfold refines_to_same in *;
+        simpl in *; cleanup.
+        2: {
+          exists(u,o,dh,s); split.
+          simpl_refines_to; intuition.
+          instantiate (1:= (u, o, x1, s)).
+          simpl_refines_to; intuition eauto.
+        }
+        
+        simpl_refines_to; cleanup; intuition.
+        eexists; intuition.
+        eauto.
+        all: simpl in *; eauto.
+        eapply rep_trans; eauto.
+
+        eapply exec_limited_preserves_refinement in H3; unfold refines_to_same in *;
+          simpl in *; cleanup.
+         2: {
+          exists(u,o,dh,s); split.
+          simpl_refines_to; intuition.
+          eauto.
+        }
+        simpl_refines_to; cleanup; intuition.
+        eexists; intuition.
+        eauto.
+        all: simpl in *; eauto.
+        eapply rep_trans; eauto.
+    Qed.
+
+
+
+
+
+    Lemma exec_deterministic_oracle:
+      forall T (p: prog T) st1 st2 st1' st2' tr1 tr2,
+        exec st1 p st1' tr1 ->
+        exec st2 p st2' tr2 ->
+        Prog.get_oracle st1 = Prog.get_oracle st2 ->
+        Prog.get_oracle (extract_state st1') = Prog.get_oracle (extract_state st2').
+    Proof.
+      unfold Prog.get_oracle;
+        induction p; intros; simpl in *;
+          simpl_states; cleanup;
+            invert_exec; invert_exec;
+              cleanup; simpl in *;
+          cleanup; eauto;
+      try match goal with
+      |[H: _ :: _ = _ :: _ |- _] =>
+       inversion H; eauto
+      end.      
+      simpl_states; cleanup.
+   Abort.
+
+
+    
+    
+
+   
+
+
+
+    
+  
+  
+  
+
+    
+    
+    
+                                     (*
+    Lemma rep_equivalent_for_fst_high:
+      forall u d1 d2 d1' d2',
+        @equivalent_for_fst _ addr_dec _ u d2 d2' ->
+        rep d2 d1 ->
+        rep d2' d1' ->
+        @equivalent_for_fst _ addr_dec _ u d1 d1'.
+    Proof.
+      unfold equivalent_for, equivalent_for_fst, rep; intros.
+      destruct_lift H0; destruct_lift H1; cleanup.
+
+      assert_fresh (dummy = dummy1).
+      {
+        setoid_rewrite <- value_to_nat_to_value.
+      
+        destruct (value_to_nat dummy1);
+          destruct (value_to_nat dummy); intuition; cleanup.
+        destruct n; intuition; cleanup.
+        specialize (H 1) as Hx; intuition; cleanup.
+        destruct n; intuition; cleanup.
+        specialize (H 2) as Hx; intuition; cleanup.
+        destruct n; intuition; cleanup.
+        specialize (H 1) as Hx; intuition; cleanup.
+
+        destruct n; intuition; cleanup.
+        specialize (H 1) as Hx; intuition; cleanup.
+        destruct n; intuition; cleanup.
+        specialize (H 2) as Hx; intuition; cleanup.
+        destruct n; intuition; cleanup.
+        specialize (H 1) as Hx; intuition; cleanup.
+
+        destruct n; intuition; cleanup.
+        destruct n0; intuition; cleanup.
+        destruct n0; intuition; cleanup.
+        specialize (H 1) as Hx; intuition; cleanup.
+        destruct n0; intuition; cleanup.
+        specialize (H 2) as Hx; intuition; cleanup.
+        
+        destruct n; intuition; cleanup.
+        destruct n0; intuition; cleanup.
+        specialize (H 1) as Hx; intuition; cleanup.
+        destruct n0; intuition; cleanup.
+        destruct n0; intuition; cleanup.
+        specialize (H 1) as Hx; intuition; cleanup.
+
+        destruct n; intuition; cleanup.
+        destruct n0; intuition; cleanup.
+        specialize (H 2) as Hx; intuition; cleanup.
+        destruct n0; intuition; cleanup.
+        specialize (H 1) as Hx; intuition; cleanup.
+      }
+
+      cleanup.
+      
+      destruct (Compare_dec.le_lt_dec a 2); [|intuition].
+      destruct a; intuition.
+      { (* a = 0 *)
+        setoid_rewrite ptsto_valid at 3; [| pred_apply; cancel]; cleanup.     
+        setoid_rewrite ptsto_valid at 5; [| pred_apply; cancel]; cleanup.
+        right; do 2 eexists; intuition eauto.
+      }
+      
+      destruct a; intuition.
+      setoid_rewrite ptsto_valid at 3; [| pred_apply; cancel]; cleanup.     
+      setoid_rewrite ptsto_valid at 5; [| pred_apply; cancel]; cleanup.
+      right; do 2 eexists; intuition eauto.
+      simpl in *.
+        destruct Hx; cleanup.
+      erewrite ptsto_valid in H2; [| pred_apply; cancel]; cleanup.
+      
+      erewrite ptsto_valid in H2; [| pred_apply; cancel]; cleanup.
+      erewrite ptsto_valid in H3; [| pred_apply; cancel]; cleanup.
+      simpl in *; cleanup.      
+      
+      destruct (value_to_nat dummy1); [intuition|].
+      destruct n; [intuition|].
+      destruct n; [intuition|].
+      right; do 2 eexists; intuition eauto; simpl in *.
+      destruct n; [intuition|].
+      right; do 2 eexists; intuition eauto; simpl in *.
+      omega.
+    Qed.
+
+*)
